text complete in part2

doc/book/code/Part2.Par.fst
@@ -1,85 +1,162 @@
 module Part2.Par
 open FStar.Classical.Sugar
-let state : Type = int
-
-type action =
-  | Read
-  | Write
-
-let input_of : action -> Type =
-  fun a ->
-    match a with
-    | Read -> unit
-    | Write -> state
-
-let output_of : action -> Type =
-  fun a ->
-    match a with
-    | Read -> state
-    | Write -> unit
 
 noeq
-type m (a:Type) =
-  | Return : x:a -> m a
-  | DoThen : act:action ->
-             input:input_of act ->
-             continue: (output_of act -> m a) ->
-             m a
-  | Or :  m a -> m a -> m a
+type action_class = {
+  t : Type;
+  input_of : t -> Type;
+  output_of : t -> Type;
+}
 
-let return #a (x:a)
-  : m a
+//SNIPPET_START: tree$
+noeq
+type tree (acts:action_class) (a:Type) =
+  | Return : x:a -> tree acts a
+  | DoThen : act:acts.t ->
+             input:acts.input_of act ->
+             continue: (acts.output_of act -> tree acts a) ->
+             tree acts a
+  | Or :  tree acts a -> tree acts a -> tree acts a
+//SNIPPET_END: tree$
+
+//SNIPPET_START: return and bind$
+let return #acts #a (x:a)
+  : tree acts a
   = Return x
 
-let rec bind #a #b (f: m a) (g: a -> m b)
-  : m b
+let rec bind #acts #a #b (f: tree acts a) (g: a -> tree acts b)
+  : tree acts b
   = match f with
     | Return x -> g x
     | DoThen act i k ->
       DoThen act i (fun x -> bind (k x) g)
     | Or m0 m1 -> Or (bind m0 g) (bind m1 g)
-  
-let rec l_par #a #b (f:m a) (g:m b)
-  : m (a & b)
+//SNIPPET_END: return and bind$  
+
+//SNIPPET_START: par$
+let rec l_par #acts #a #b (f:tree acts a) (g:tree acts b)
+  : tree acts (a & b)
   = match f with
     | Return v -> x <-- g; return (v, x)
     | DoThen a i k ->
       DoThen a i (fun x -> r_par (k x) g)
     | Or m0 m1 -> Or (l_par m0 g) (l_par m1 g)
 
-and r_par #a #b (f:m a) (g: m b)
-  : m (a & b)
+and r_par #acts #a #b (f:tree acts a) (g: tree acts b)
+  : tree acts (a & b)
   = match g with
     | Return v -> x <-- f; return (x, v)
     | DoThen a i k ->
       DoThen a i (fun x -> l_par f (k x))
-    | Or m0 m1 -> Or (r_par f m0) (l_par f m1)
+    | Or m0 m1 -> Or (r_par f m0) (r_par f m1)
 
-let par #a #b (f: m a) (g: m b)
-  : m (a & b)
+let par #acts #a #b (f: tree acts a) (g: tree acts b)
+  : tree acts (a & b)
   = Or (l_par f g) (r_par f g)
+//SNIPPET_END: par$
 
+////////////////////////////////////////////////////////////////////////////////
+
+type rw =
+  | Read
+  | Write
+
+let input_of : rw -> Type =
+  fun a ->
+    match a with
+    | Read -> unit
+    | Write -> int
+
+let output_of : rw -> Type =
+  fun a ->
+    match a with
+    | Read -> int
+    | Write -> unit
+
+let rw_actions = { t = rw; input_of ; output_of }
+
+//SNIPPET_START: interp$
 let randomness = nat -> bool
-let par_st a = randomness -> pos:nat -> s0:state -> (a & state & nat)
-let rec interp #a (f:m a) 
+let par_st a = randomness -> pos:nat -> s0:int -> (a & int & nat)
+let rec interp #a (f:tree rw_actions a) 
+  : par_st a 
+  = fun rand pos s0 ->
+      match f with
+      | Return x -> x, s0, pos
+      | DoThen Read _ k -> interp (k s0) rand pos s0
+      | DoThen Write s1 k -> interp (k ()) rand pos s1      
+      | Or l r -> 
+        if rand pos
+        then interp l rand (pos + 1) s0
+        else interp r rand (pos + 1) s0
+let st a = int -> a & int
+let interpret #a (f:tree rw_actions a) 
+  : st a    
+  = fun s0 -> 
+      let x, s, _ = interp f (fun n -> n % 2 = 0) 0 s0 in 
+      x, s
+//SNIPPET_END: interp$
+
+//SNIPPET_START: sample program$
+let read : tree rw_actions int = DoThen Read () Return
+let write (x:int) : tree rw_actions unit = DoThen Write x Return
+let inc
+  : tree rw_actions unit
+  = x <-- read ;
+    write (x + 1)
+let par_inc = par inc inc 
+//SNIPPET_END: sample program$
+
+//SNIPPET_START: test_par_inc$
+let test_prog = assert_norm (forall x. snd (interpret par_inc x) == x + 1)
+//SNIPPET_END: test_par_inc$
+
+//SNIPPET_START: atomic increment$
+type rwi =
+  | R
+  | W
+  | Inc
+  
+let input_of_rwi : rwi -> Type =
+  fun a ->
+    match a with
+    | R -> unit
+    | W -> int
+    | Inc -> unit
+
+let output_of_rwi : rwi -> Type =
+  fun a ->
+    match a with
+    | R -> int
+    | W -> unit
+    | Inc -> unit
+
+let rwi_actions = { t = rwi; input_of=input_of_rwi ; output_of=output_of_rwi }
+
+let atomic_inc : tree rwi_actions unit = DoThen Inc () Return
+
+let rec interp_rwi #a (f:tree rwi_actions a) 
   : par_st a 
   = fun tape pos s0 ->
       match f with
       | Return x -> x, s0, pos
-      | DoThen Read _ k -> interp (k s0) tape pos s0
-      | DoThen Write s1 k -> interp (k ()) tape pos s1      
+      | DoThen R _ k -> interp_rwi (k s0) tape pos s0
+      | DoThen W s1 k -> interp_rwi (k ()) tape pos s1      
+      | DoThen Inc () k -> interp_rwi (k ()) tape pos (s0 + 1)            
       | Or l r -> 
         let b = tape pos in
         if b
-        then interp l tape (pos + 1) s0
-        else interp r tape (pos + 1) s0
+        then interp_rwi l tape (pos + 1) s0
+        else interp_rwi r tape (pos + 1) s0
+let interpret_rwi #a (f:tree rwi_actions a) 
+  : st a    
+  = fun s0 -> 
+      let x, s, _ = interp_rwi f (fun n -> n % 2 = 0) 0 s0 in 
+      x, s
 
-let tape = fun n -> n%2 = 0
-let read : m state = DoThen Read () Return
-let write (x:state) : m unit = DoThen Write x Return
-let inc
-  : m unit
-  = x <-- read ;
-    write (x + 1)
+let par_atomic_inc = par atomic_inc atomic_inc
+let test_par_atomic_inc = assert_norm (forall x. snd (interpret_rwi par_atomic_inc x) == x + 2)
+//SNIPPET_END: atomic increment$
 
-let prog = par inc inc //interprets to 1
+
+
