doc/book/code/Part2.FreeFunExt.fst
@@ -1,46 +1,31 @@
-module Part2.Free
+module Part2.FreeFunExt
 open FStar.Classical.Sugar
+module F = FStar.FunctionalExtensionality
+open FStar.FunctionalExtensionality
 
-//SNIPPET_START: action_class$
 noeq
 type action_class = {
   t : Type;
   input_of : t -> Type;
   output_of : t -> Type;
 }
-//SNIPPET_END: action_class$
 
-//SNIPPET_START: rw_action_class$
-type rw =
-  | Read
-  | Write
 
-let input_of : rw -> Type =
-  fun a ->
-    match a with
-    | Read -> unit
-    | Write -> int
-
-let output_of : rw -> Type =
-  fun a ->
-    match a with
-    | Read -> int
-    | Write -> unit
-
-let rw_action_class = { t = rw; input_of ; output_of }
-//SNIPPET_END: rw_action_class$
-
-//SNIPPET_START: tree$
+// A F* elaborator bug prevents typechecking the auto-generated projector 
+// for DoThen?.continue. This options disables the feature. 
+// A fix for this long-standing issue is discussed in issue #1355
+#push-options "--__temp_no_proj Part2.FreeFunExt"
 noeq
 type tree (acts:action_class) (a:Type) =
   | Return : x:a -> tree acts a
   | DoThen : act:acts.t ->
              input:acts.input_of act ->
-             continue: (acts.output_of act -> tree acts a) ->
+             //We have to restrict continuations to be eta expanded
+             //that what `^->` does. Its defined in FStar.FunctionalExtensionality
+             continue:(acts.output_of act ^-> tree acts a) ->
              tree acts a
-//SNIPPET_END: tree$
+#pop-options
 
-//SNIPPET_START: return and bind$
 let return #a #acts (x:a)
   : tree acts a
   = Return x
@@ -50,10 +35,10 @@ let rec bind #acts #a #b (f: tree acts a) (g: a -> tree acts b)
   = match f with
     | Return x -> g x
     | DoThen act i k ->
-      DoThen act i (fun x -> bind (k x) g)
-//SNIPPET_END: return and bind$
+      //Now, we have to ensure that continuations are instances of
+      //F.( ^-> )
+      DoThen act i (F.on _ (fun x -> bind (k x) g))
 
-//SNIPPET_START: equiv$
 let rec equiv #acts #a (x y: tree acts a) =
   match x, y with 
   | Return vx, Return vy -> vx == vy
@@ -62,9 +47,7 @@ let rec equiv #acts #a (x y: tree acts a) =
     ix == iy /\
     (forall o. equiv (kx o) (ky o))
   | _ -> False
-//SNIPPET_END: equiv$
 
-//SNIPPET_START: equiv is an equivalence$
 let rec equiv_refl #acts #a (x:tree acts a) 
   : Lemma (equiv x x)
   = match x with
@@ -92,10 +75,19 @@ let rec equiv_trans #acts #a (x y z: tree acts a)
     | DoThen act i kx, DoThen _ _ ky, DoThen _ _ kz ->
       introduce forall o. equiv (kx o) (kz o)
       with equiv_trans (kx o) (ky o) (kz o)
-//SNIPPET_END: equiv is an equivalence$  
 
+// THIS IS THE MAIN LEMMA OF THE EXERCISE
+let rec equiv_is_equal #acts #a (x y: tree acts a)
+  : Lemma
+    (requires equiv x y)
+    (ensures x == y)
+  = match x, y with
+    | Return _, Return _ -> ()
+    | DoThen act i kx, DoThen _ _ ky ->
+      introduce forall o. kx o == ky o
+      with equiv_is_equal (kx o) (ky o);
+      F.extensionality _ _ kx ky
 
-//SNIPPET_START: tree is a monad$
 let right_identity #acts #a #b (x:a) (g:a -> tree acts b)
   : Lemma (bind (return x) g `equiv` g x)
   = equiv_refl (g x)
@@ -122,19 +114,34 @@ let rec assoc #acts #a #b #c
       introduce forall o. bind (k o) (fun x -> bind (f2 x) f3) `equiv`
                      bind (bind (k o) f2) f3
       with assoc (k o) f2 f3
-//SNIPPET_END: tree is a monad$
 
-//SNIPPET_START: read_and_increment$
-let read : tree rw_action_class int = DoThen Read () Return
-let write (x:int) : tree rw_action_class unit = DoThen Write x Return
+type rw =
+  | Read
+  | Write
+
+let input_of : rw -> Type =
+  fun a ->
+    match a with
+    | Read -> unit
+    | Write -> int
+
+let output_of : rw -> Type =
+  fun a ->
+    match a with
+    | Read -> int
+    | Write -> unit
+
+let rw_action_class = { t = rw; input_of ; output_of }
+
+//Here again the continuation has to be F.( ^-> )
+let read : tree rw_action_class int = DoThen Read () (F.on _ Return) 
+let write (x:int) : tree rw_action_class unit = DoThen Write x (F.on _ Return)
 let read_and_increment 
   : tree rw_action_class int
   = x <-- read ;
     write (x + 1);;
     return x
-//SNIPPET_END: read_and_increment$
 
-//SNIPPET_START: interp$
 let st a = int -> a & int
 let rec interp #a (f: tree rw_action_class a)
   : st a 
@@ -145,17 +152,11 @@ let rec interp #a (f: tree rw_action_class a)
        interp (k s0) s0
      | DoThen Write s1 k -> 
        interp (k ()) s1
-//SNIPPET_END: interp$       
 
-//SNIPPET_START: interp_equiv$       
-let feq #a #b (f g: a -> b) = forall x. f x == g x
-let rec interp_equiv #a (f g:tree rw_action_class a)
+// And now since equivalent trees and equal, lemmas such as this
+// become trivial
+let interp_equiv #a (f g:tree rw_action_class a)
   : Lemma
     (requires equiv f g)
     (ensures feq (interp f) (interp g))
-  = match f, g with
-    | Return _, Return _ -> ()
-    | DoThen act i kf, DoThen _ _ kg ->
-      introduce forall o. feq (interp (kf o)) (interp (kg o))
-      with interp_equiv (kf o) (kg o)
-//SNIPPET_END: interp_equiv$       
+  = equiv_is_equal f g
